reestablishing the invariant with the changed style in MasterSecret

src/tls/ConnInvariant.fst
@@ -38,19 +38,34 @@ let registered (i:id{StAE.is_stream_ae i}) (w:StreamAE.writer i) (c:connection) 
       (let i' = Handshake.hsId (Handshake.Epoch.h e) in
         i=i' /\ StAE.stream_ae #i e.w == w))
 
+let ms_conn_inv (ms:ms_tab)
+ 		(conn:c_tab)
+		(h:HyperHeap.t) 
+		(i:id) 
+   = authId i /\ StAE.is_stream_ae i ==>  //Focused only on TLS-1.3 for now, hence the is_stream_ae guard
+     (match MM.sel ms i with 
+      | None -> True
+      | Some w -> 
+	Map.contains h (StreamAE.State.region w) /\ //technical for framing; need to know that the writer's region exists
+	HH.disjoint (StreamAE.State.region w) tls_tables_region /\
+	(MR.m_sel h (StreamAE.ilog (StreamAE.State.log w)) = Seq.createEmpty  \/   //the writer is still unused; or
+	             (let copt = MM.sel conn (I.nonce_of_id i) in
+  		      is_Some copt /\ registered i w (Some.v copt) h)))      //it's been assigned to a connection
+
 let ms_conn_invariant (ms:ms_tab)
  		      (conn:c_tab)
 		      (h:HyperHeap.t) 
-  = forall (i:id) .{:pattern (MM.sel ms i)}
-	     authId i /\ StAE.is_stream_ae i ==>  //Focused only on TLS-1.3 for now, hence the is_stream_ae guard
-	            (match MM.sel ms i with 
-		     | None -> True
-		     | Some w -> 
-		       Map.contains h (StreamAE.State.region w) /\ //technical for framing; need to know that the writer's region exists
- 		       (MR.m_sel h (StreamAE.ilog (StreamAE.State.log w)) = Seq.createEmpty  \/   //the writer is still unused; or
-		        False))
-		        (* (let copt = MM.sel conn (I.nonce_of_id i) in *)
-  			(*  is_Some copt /\ registered i w (Some.v copt) h)))      //it's been assigned to a connection *)
+  = forall (i:id) .{:pattern (MM.sel ms i)} ms_conn_inv ms conn h i
+  
+	     (* authId i /\ StAE.is_stream_ae i ==>  //Focused only on TLS-1.3 for now, hence the is_stream_ae guard *)
+	     (*        (match MM.sel ms i with  *)
+	     (* 	     | None -> True *)
+	     (* 	     | Some w ->  *)
+	     (* 	       Map.contains h (StreamAE.State.region w) /\ //technical for framing; need to know that the writer's region exists *)
+ 	     (* 	       (MR.m_sel h (StreamAE.ilog (StreamAE.State.log w)) = Seq.createEmpty  \/   //the writer is still unused; or *)
+	     (* 	        False)) *)
+	     (* 	        (\* (let copt = MM.sel conn (I.nonce_of_id i) in *\) *)
+  	     (* 		(\*  is_Some copt /\ registered i w (Some.v copt) h)))      //it's been assigned to a connection *\) *)
 
 let mc_inv (h:HyperHeap.t) = ms_conn_invariant (MR.m_sel h MS.ms_tab) (MR.m_sel h conn_table) h
 
@@ -58,8 +73,8 @@ let mc_inv (h:HyperHeap.t) = ms_conn_invariant (MR.m_sel h MS.ms_tab) (MR.m_sel 
 
 //1. Deriving a new key involves adding a new writer to the ms table (because we tried a lookup at id and it failed)
 //   Easy: because a new log is empty and both cases of the conn table allow empty logs to be in ms
- 
-val ms_derive_is_ok: h0:HyperHeap.t -> h1:HyperHeap.t -> i:id -> w:MS.writer i
+
+val ms_derive_is_ok': h0:HyperHeap.t -> h1:HyperHeap.t -> i:id -> w:MS.writer i -> j:id
   -> Lemma (requires 
 		 HH.contains_ref (MR.as_rref conn_table) h0 /\
 		 HH.contains_ref (MR.as_rref MS.ms_tab) h0 /\
@@ -73,68 +88,85 @@ val ms_derive_is_ok: h0:HyperHeap.t -> h1:HyperHeap.t -> i:id -> w:MS.writer i
 		 (let old_ms = MR.m_sel h0 MS.ms_tab in 
 		  let new_ms = MR.m_sel h1 MS.ms_tab in
 		  MM.sel old_ms i = None /\
-		  new_ms = MM.upd old_ms i w) /\                                    and the ms_tab only changed by adding w
+		  new_ms = MM.upd old_ms i w) /\                                    //and the ms_tab only changed by adding w
 		 MR.m_sel h1 (StreamAE.ilog (StreamAE.State.log w)) = Seq.createEmpty)             //and w's log is empty
-	 (ensures mc_inv h1)                                                       //we're back in the invariant
-let ms_derive_is_ok h0 h1 i w = ()
+	 (ensures (
+		  let new_ms = MR.m_sel h1 MS.ms_tab in
+		  let new_conn = MR.m_sel h1 conn_table in
+		  ms_conn_inv new_ms new_conn h1 j))
+	 (* mc_inv h1)                                                       //we're back in the invariant *)
+let ms_derive_is_ok' h0 h1 i w j = 
+  let old_ms = MR.m_sel h0 MS.ms_tab in 
+  let new_ms = MR.m_sel h1 MS.ms_tab in
+  let new_conn = MR.m_sel h1 conn_table in
+  assert (ms_conn_inv new_ms new_conn h1 i);
+  if (authId j && StAE.is_stream_ae j)
+  then match MM.sel new_ms j with 
+       | None -> ()
+       | Some ww -> 
+	 if ww=w 
+	 then ()
+	 else assert (Some ww=MM.sel old_ms j)
+  else ()
 
-//2. Adding a new epoch to a connection c, with a fresh index (hdId i) for c
-//      -- we found a writer w at (ms i), pre-allocated (we're second) or not (we're first)
-//      -- we need to show that the (exists e. SeqProperties.mem ...) is false (because of the fresh index for c)
-//      -- so, we're in the "not yet used" case ... so, the epoch's writer is in its initial state and we can return it (our goal is to return a fresh epoch)
-val add_epoch_ok: h0:HyperHeap.t -> h1:HyperHeap.t -> i:id{StAE.is_stream_ae i /\ authId i} 
-		-> c:r_conn (idNonce i) -> e:epoch (HS.region c.hs) (HS.peer c.hs) 
-  -> Lemma (requires 
-            (let ctab = MR.m_sel h0 conn_table in
-	     let mstab = MR.m_sel h0 MS.ms_tab in
-	     let old_hs_log = HH.sel h0 (HS.log c.hs) in
-     	     let new_hs_log = HH.sel h1 (HS.log c.hs) in 
-	     let rgn = HS.region c.hs in
-	     HH.contains_ref (MR.as_rref conn_table) h0 /\
-	     HH.contains_ref (MR.as_rref MS.ms_tab) h0 /\
-	     HH.disjoint (HS.region c.hs) tls_region /\
-	     HH.contains_ref (HS.log c.hs) h0 /\
-	     HH.contains_ref (HS.log c.hs) h1 /\
-	     mc_inv h0 /\ //we're initially in the invariant
-	     i=hsId (Epoch.h e) /\ //the epoch has id it
-	     (let w = StAE.stream_ae #i (Epoch.w e) in //the epoch writer
-	      let epochs = HH.sel h0 (HS.log c.hs) in
-      	      Map.contains h1 (StreamAE.State.region w) /\
-	      (forall e. SeqProperties.mem e epochs ==> hsId (Epoch.h e) <> i) /\ //i is fresh for c
- 	      MM.sel mstab (i, rgn) = Some w /\ //we found the writer in the ms_tab
-	      MM.sel ctab (idNonce i) = Some c /\ //we found the connection in the conn_table
-	      HH.modifies_one (HS.region c.hs) h0 h1 /\ //we just modified this connection's handshake region
-	      HH.modifies_rref (HS.region c.hs) !{HH.as_ref (HS.log c.hs)} h0 h1 /\ //and within it, just the epochs log
-	      new_hs_log = SeqProperties.snoc old_hs_log e))) //and we modified it by adding this epoch to it
-	  (ensures mc_inv h1) //we're back in the invariant
 
-#reset-options "--z3timeout 10 --initial_fuel 2 --max_fuel 2 --initial_ifuel 2 --max_ifuel 2"
+(* //2. Adding a new epoch to a connection c, with a fresh index (hdId i) for c *)
+(* //      -- we found a writer w at (ms i), pre-allocated (we're second) or not (we're first) *)
+(* //      -- we need to show that the (exists e. SeqProperties.mem ...) is false (because of the fresh index for c) *)
+(* //      -- so, we're in the "not yet used" case ... so, the epoch's writer is in its initial state and we can return it (our goal is to return a fresh epoch) *)
+(* val add_epoch_ok: h0:HyperHeap.t -> h1:HyperHeap.t -> i:id{StAE.is_stream_ae i /\ authId i}  *)
+(* 		-> c:r_conn (idNonce i) -> e:epoch (HS.region c.hs) (HS.peer c.hs)  *)
+(*   -> Lemma (requires  *)
+(*             (let ctab = MR.m_sel h0 conn_table in *)
+(* 	     let mstab = MR.m_sel h0 MS.ms_tab in *)
+(* 	     let old_hs_log = HH.sel h0 (HS.log c.hs) in *)
+(*      	     let new_hs_log = HH.sel h1 (HS.log c.hs) in  *)
+(* 	     let rgn = HS.region c.hs in *)
+(* 	     HH.contains_ref (MR.as_rref conn_table) h0 /\ *)
+(* 	     HH.contains_ref (MR.as_rref MS.ms_tab) h0 /\ *)
+(* 	     HH.disjoint (HS.region c.hs) tls_region /\ *)
+(* 	     HH.contains_ref (HS.log c.hs) h0 /\ *)
+(* 	     HH.contains_ref (HS.log c.hs) h1 /\ *)
+(* 	     mc_inv h0 /\ //we're initially in the invariant *)
+(* 	     i=hsId (Epoch.h e) /\ //the epoch has id it *)
+(* 	     (let w = StAE.stream_ae #i (Epoch.w e) in //the epoch writer *)
+(* 	      let epochs = HH.sel h0 (HS.log c.hs) in *)
+(*       	      Map.contains h1 (StreamAE.State.region w) /\ *)
+(* 	      (forall e. SeqProperties.mem e epochs ==> hsId (Epoch.h e) <> i) /\ //i is fresh for c *)
+(*  	      MM.sel mstab (i, rgn) = Some w /\ //we found the writer in the ms_tab *)
+(* 	      MM.sel ctab (idNonce i) = Some c /\ //we found the connection in the conn_table *)
+(* 	      HH.modifies_one (HS.region c.hs) h0 h1 /\ //we just modified this connection's handshake region *)
+(* 	      HH.modifies_rref (HS.region c.hs) !{HH.as_ref (HS.log c.hs)} h0 h1 /\ //and within it, just the epochs log *)
+(* 	      new_hs_log = SeqProperties.snoc old_hs_log e))) //and we modified it by adding this epoch to it *)
+(* 	  (ensures mc_inv h1) //we're back in the invariant *)
 
-let add_epoch_ok h0 h1 i c e = 
-  assert (MR.m_sel h0 MS.ms_tab = MR.m_sel h1 MS.ms_tab);
-  assert (MR.m_sel h0 conn_table = MR.m_sel h1 conn_table);
-  let w = StAE.stream_ae #i (Epoch.w e) in //the epoch writer
-  assert (MR.m_sel h0 (StreamAE.ilog (StreamAE.State.log w)) = MR.m_sel h1 (StreamAE.ilog (StreamAE.State.log w)));
-  let ctab = MR.m_sel h0 conn_table in
-  let mstab = MR.m_sel h0 MS.ms_tab in
-  let copt = MM.sel ctab (idNonce i) in
-  let old_hs_log = HH.sel h0 (HS.log c.hs) in
-  assert (is_Some copt);
-  assert (~ (registered i w (Some.v copt) h0));
-  MonotoneSeq.lemma_mem_snoc old_hs_log e;
-  assert (registered i w (Some.v copt) h1);
-  let j : id  = magic () in 
-  let s : HH.rid = magic () in 
-  assume (StAE.is_stream_ae j);
-  assume (authId j);
-  assume (s <> HS.region c.hs);
-  match MM.sel mstab (j, s) with 
-  | None -> admit()
-  | Some wj -> 
-    assume (StreamAE.State.region wj <> HS.region c.hs); //can see here why the post-condition fails ... need better separation invariants between the HS.log and the writer logs
-    assume (HH.contains_ref (MR.as_rref (StreamAE.ilog (StreamAE.State.log wj))) h0);
-    assert (MR.m_sel h0 (StreamAE.ilog (StreamAE.State.log wj)) = MR.m_sel h1 (StreamAE.ilog (StreamAE.State.log wj)));
-    admit()
+(* #reset-options "--z3timeout 10 --initial_fuel 2 --max_fuel 2 --initial_ifuel 2 --max_ifuel 2" *)
+
+(* let add_epoch_ok h0 h1 i c e =  *)
+(*   assert (MR.m_sel h0 MS.ms_tab = MR.m_sel h1 MS.ms_tab); *)
+(*   assert (MR.m_sel h0 conn_table = MR.m_sel h1 conn_table); *)
+(*   let w = StAE.stream_ae #i (Epoch.w e) in //the epoch writer *)
+(*   assert (MR.m_sel h0 (StreamAE.ilog (StreamAE.State.log w)) = MR.m_sel h1 (StreamAE.ilog (StreamAE.State.log w))); *)
+(*   let ctab = MR.m_sel h0 conn_table in *)
+(*   let mstab = MR.m_sel h0 MS.ms_tab in *)
+(*   let copt = MM.sel ctab (idNonce i) in *)
+(*   let old_hs_log = HH.sel h0 (HS.log c.hs) in *)
+(*   assert (is_Some copt); *)
+(*   assert (~ (registered i w (Some.v copt) h0)); *)
+(*   MonotoneSeq.lemma_mem_snoc old_hs_log e; *)
+(*   assert (registered i w (Some.v copt) h1); *)
+(*   let j : id  = magic () in  *)
+(*   let s : HH.rid = magic () in  *)
+(*   assume (StAE.is_stream_ae j); *)
+(*   assume (authId j); *)
+(*   assume (s <> HS.region c.hs); *)
+(*   match MM.sel mstab (j, s) with  *)
+(*   | None -> admit() *)
+(*   | Some wj ->  *)
+(*     assume (StreamAE.State.region wj <> HS.region c.hs); //can see here why the post-condition fails ... need better separation invariants between the HS.log and the writer logs *)
+(*     assume (HH.contains_ref (MR.as_rref (StreamAE.ilog (StreamAE.State.log wj))) h0); *)
+(*     assert (MR.m_sel h0 (StreamAE.ilog (StreamAE.State.log wj)) = MR.m_sel h1 (StreamAE.ilog (StreamAE.State.log wj))); *)
+(*     admit() *)
 
 
 //3. Adding to a log registered in a connection: Need to prove that ms_conn_invariant is maintained
